\documentclass[8pt]{amsart}
\usepackage{amsmath, amssymb}
\usepackage{amsfonts}
\usepackage{mathrsfs}
\usepackage[arrow,matrix,curve,cmtip,ps]{xy}
\usepackage{paralist}
\usepackage[left=1in,top=1in,right=1in,bottom=1in]{geometry}
\usepackage{amsthm}
\usepackage{tikz}
\usetikzlibrary{arrows,chains,matrix,positioning,scopes}

\allowdisplaybreaks

\theoremstyle{plain}% default

\theoremstyle{definition}
\newtheorem{theorem}{Theorem}[section]
\newtheorem{lemma}{Lemma}[section]
\newtheorem*{proposition}{Proposition}
\newtheorem*{corollary}{Corollary}
\newtheorem*{KL}{Kleinâ€™s Lemma}

\newtheorem*{definition}{Definition}
\newtheorem{conjecture}{Conjecture}[section]
\newtheorem{example}{Example}[section]
\newtheorem*{exercise}{Exercise}%[section]
\newtheorem*{notation}{Notation}
\newtheorem*{remark}{Remark}

\theoremstyle{remark}
\newtheorem*{note}{Note}
\newtheorem{case}{Case}

%this has equations numbered within sections 1.1,1.2, ... 2.1,...
\numberwithin{equation}{section}

\makeatletter
\newenvironment{solution}
               {\let\oldqedsymbol=\qedsymbol%
                \def\@addpunct##1{}%
                \renewcommand{\qedsymbol}{$\blacktriangleleft$}%
                \begin{proof}[\itshape Solution.]}%
               {\end{proof}%
                \renewcommand{\qedsymbol}{\oldqedsymbol}}
\makeatother

\makeatletter
\tikzset{join/.code=\tikzset{after node path={%
\ifx\tikzchainprevious\pgfutil@empty\else(\tikzchainprevious)%
edge[every join]#1(\tikzchaincurrent)\fi}}}
\makeatother

\tikzset{>=stealth',every on chain/.append style={join},
         every join/.style={->}}




\def\upint{\mathchoice%
    {\mkern13mu\overline{\vphantom{\intop}\mkern7mu}\mkern-20mu}%
    {\mkern7mu\overline{\vphantom{\intop}\mkern7mu}\mkern-14mu}%
    {\mkern7mu\overline{\vphantom{\intop}\mkern7mu}\mkern-14mu}%
    {\mkern7mu\overline{\vphantom{\intop}\mkern7mu}\mkern-14mu}%
  \int}
\def\lowint{\mkern3mu\underline{\vphantom{\intop}\mkern7mu}\mkern-10mu\int}


%-------------------------------------------
%       Begin Local Macros
%-------------------------------------------

\newcommand{\Z}{\mathbb{Z}}
\newcommand{\N}{\mathbb{N}}
\newcommand{\Q}{\mathbb{Q}}
\newcommand{\R}{\mathbb{R}}
\newcommand{\C}{\mathbb{C}}
\newcommand{\T}{\mathbb{T}}
\newcommand{\D}{\displaystyle}
\newcommand{\im}{\operatorname{im}}
\newcommand{\coker}{\operatorname{coker}}
\newcommand{\obj}{\operatorname{obj}}
\newcommand{\Hom}{\operatorname{Hom}}
\newcommand{\Mod}{\operatorname{\textbf{Mod}}}
\newcommand{\ind}{\operatorname{ind}}
\newcommand{\rank}{\operatorname{rank}}
\newcommand\mc[1]{\marginpar{\sloppy\protect\footnotesize #1}}

%-------------------------------------------
%       End Local Macros
%-------------------------------------------
\begin{document}
\title[MATH 697]{Introduction to Homological Algebra}

% \author{Robert Cardona}

\author{
	Robert Cardona %\textit{mrrobertcardona@gmail.com}
	\and
	Massy Khoshbin %\textit{massy255@gmail.com}
	\and
	Siavash Mortezavi %\textit{siavash.mortezavi@gmail.com}
}


\address{Department of Mathematics \\ California State University Long Beach}
\email{mrrobertcardona@gmail.com \and massy255@gmail.com \and siavash.mortezavi@gmail.com}

\date{\today}


\maketitle

%%%%%%%%%%%%%%%%%%%%%%%%%%%%%%%%%%%%%%%%%%%%%%%%
\setcounter{section}{0}
\section{MATH 697 Notes}
%%%%%%%%%%%%%%%%%%%%%%%%%%%%%%%%%%%%%%%%%%%%%%%%

A \textbf{category} $C$ consists of three ingredients: a class $\obj(C)$ of \textbf{objects}, a set of \textbf{morphisms} $\Hom(A, B)$ for every ordered pair $(A, B)$ of objects, and \textbf{composition} $\Hom(A, B) \times \Hom(B, C) \to \Hom(A, C)$, denoted by $(f, g) \mapsto gf$. for every ordered triple $A, B, C$ of objects. These ingredients are subject to the following axioms:
	\begin{enumerate}
		\item The Hom sets are pairwise disjoint; that is, each $f \in \Hom(A, B)$ has a unique \textbf{domain} $A$ and a unique \textbf{target} $B$.
		\item For each object $A$, there is an \textbf{identity morphism} $1_A \in \Hom(A, A)$ such that $f1_A = f$ and $1_Bf = f$ for all $f : A \to B$.
		\item Composition is associative: given morphisms $A \xrightarrow f B \xrightarrow g C \xrightarrow h D$, then $h(fg) = (hg)f$.\\
	\end{enumerate}

Examples of categories: \textbf{Sets}, \textbf{Groups}, \textbf{Top}, \textbf{Ab}, \textbf{Rings}, \textbf{ComRings}.\\

A \textbf{left $R$-module}, where $R$ is a ring, is an additive abelian group $M$ having a \textit{scalar multiplication} $R \times M \to M$, denoted by $(r, m) \mapsto rm$, such that, for all $m, m' \in M$ and $r, r' \in R$. We often write $_RM$ to denote $M$ being a left $R$-module.
	\begin{enumerate}
		\item $r(m + m') = rm + rm'$
		\item $(r + r')m = rm + r'm$
		\item $(rr')m = r(r'm)$
		\item $1m = m$.\\
	\end{enumerate}

If $M$ and $N$ are left $R$-modules, then an $R$-\textbf{homomorphism} (or an $R$-\textbf{map}) is a function $f : M \to N$ such that, for all $m, m' \in M$ and $r \in R$,
	\begin{enumerate}
		\item $f(m + m') = f(m) + f(m')$
		\item $f(rm) = r(fm)$\\
	\end{enumerate}

An $R$-\textbf{isomorphism} is a bijective $R$-homomorphism.\\

A \textbf{right $R$-module}, where $R$ is a ring, is an additive abelian group $M$ having a \textit{scalar multiplication} $M \times R \to M$, denoted by $(m, r) \mapsto mr$, such that, for all $m, m' \in M$ and $r, r' \in R$. We often write $M_R$ to denote $M$ being a right $R$-module.
	\begin{enumerate}
		\item $(m + m')r = mr + m'r$
		\item $m(r + r') = mr + mr'$
		\item $m(rr') = (mr)r'$
		\item $m = m1$\\
	\end{enumerate}

The category $_R\Mod$ of all \textbf{left $R$-modules} (where $R$ is a ring) has as its objects all left $R$-modules, has as its morphisms all $R$-homomorphisms, and as its composition the usual composition of functions. We denote the sets $\Hom(A, B)$ in $_R\Mod$ by $\Hom_R(A, B)$.\\

The category $\Mod_R$ of all \textbf{right $R$-modules} (where $R$ is a ring) has as its objects all \textbf{right $R$-modules}, as its morphisms all $R$-homomorphisms, and as its composition the usual composition. We denote the sets $\Hom(A, B)$ in $\Mod_R$ by $\Hom_R(A, B)$.\\

A category $S$ is a \textbf{subcategory} of a category $C$ if
	\begin{enumerate}
		\item $\obj(S) \subseteq \obj(C)$
	\end{enumerate}


\textbf{R Proposition 2.18}:
	\begin{enumerate}
		\item A sequence $0 \rightarrow A \xrightarrow{f} B$ is exact if and only if $f$ is injective.
		\item A sequence $B \xrightarrow g C \rightarrow 0$ is exact if and only if $g$ is surjective.
		\item A sequence $0 \rightarrow A \xrightarrow{h} B \rightarrow 0$ is exact if and only if $h$ is an isomorphism.
	\end{enumerate}

\textbf{DF \S10.5 Proposition 24}: (\textit{The Short Five Lemma}) Let $\alpha, \beta, \gamma$ be homomorphisms of short exact sequences:\\

	\begin{center}
	\begin{tikzpicture}
	  \matrix (m) [matrix of math nodes, row sep=3em, column sep=3em]
	    { 0 & A  & B  & C  & 0 \\
	      0 & A' & B' & C' & 0 \\ };
	  { [start chain] \chainin (m-1-1);
	    \chainin (m-1-2);
	    { [start branch=A] \chainin (m-2-2)
	        [join={node[right] {$\scriptstyle\alpha$}}];}
	    \chainin (m-1-3) [join={node[above] {$\scriptstyle f$}}];
	    { [start branch=B] \chainin (m-2-3)
	        [join={node[right] {$\scriptstyle\beta$}}];}
	    \chainin (m-1-4) [join={node[above] {$\scriptstyle g$}}];
	    { [start branch=C] \chainin (m-2-4)
	        [join={node[right] {$\scriptstyle\gamma$}}];}
	    \chainin (m-1-5); }
	  { [start chain] \chainin (m-2-1);
	    \chainin (m-2-2);
	    \chainin (m-2-3) [join={node[above] {$\scriptstyle f'$}}];
	    \chainin (m-2-4) [join={node[above] {$\scriptstyle g'$}}];
	    \chainin (m-2-5); }
	\end{tikzpicture}
	\end{center}

	\begin{enumerate}
		\item If $\alpha$ and $\gamma$ are injective then so is $\beta$.
			\begin{proof}
				Let $b \in B$ such that $\beta(b) = 0$. We want to show that $b = 0$. Observe that $g'(\beta(b)) = g'(0) = 0$. By commutativity we have $\gamma(g(b)) = g'(\beta(b)) = g'(0) = 0$. Since $\gamma$ is injective we know $g(b) = 0$ so $b \in \ker g$ but since we are in an exact sequence we have $\im f = \ker g$ and hence $b \in \im f$. By definition there exists $a \in A$ with $f(a) = b$. Now $f'(\alpha(a)) = \beta(f(a)) = \beta(b) = 0$. Since $f'$ is injective, it follows that $\alpha(a) = (f')^{-1}(0) = 0$. Now we have $a = \alpha^{-1}(0)$ and so $a = 0$. So $0 = f(a) = b$.
			\end{proof}
		\item If $\alpha$ and $\gamma$ are surjective then so is $\beta$.
			\begin{proof}
				Let $b' \in B'$ then $g'(b') \in C'$. Since $\gamma$ is surjective there excists $c \in C$ such that $\gamma(c) = g'(b')$. Since this is an exact sequence, $g$ is surjective so there exists $b \in B$ such that $g(b) = c$. By equality we have $\gamma(c) = \gamma(g(b)) = g'(b')$. Now observe that $$g'(b' - \beta(b)) = g'(b') - g'(\beta(b)) = g'(b') - \gamma(g(b)) = g'(b') - g'(b') = 0$$ So in particular $b' - \beta(b) \in \ker g'$ but by exactness $\im f' = \ker g'$ so there exists $a' \in A'$ such that $f'(a') = b' - \beta(b)$. But since $\alpha$ is surjective, there exists $a \in A$ such that $\alpha(a) = a'$. Now $f'(a') = f'(\alpha(a)) = b' - \beta(b)$. By commutativity $f'(\alpha(a)) = \beta(f(a)) = b' - \beta(b)$ so $\beta(f(a)) + \beta(b) = b'$ and we have $\beta(f(a) + b) = b'$.
			\end{proof}
		\item If $\alpha$ and $\gamma$ are isomorphisms then so is $\beta$ (and then the two sequences are isomorphism).
			\begin{proof}
				Follows from $(1)$ and $(2)$.\\
			\end{proof}
	\end{enumerate}

\textbf{R Proposition 2.72}: (\textit{Five Lemma}) Consider the commutative diagram with exact rows.
	\begin{center}
	\begin{tikzpicture}
	  \matrix (m) [matrix of math nodes, row sep=3em, column sep=3em]
	    { A_1 & A_2  & A_3  & A_4  & A_5 \\
	      B_1 & B_2 & B_3 & B_4 & B_5 \\ };
	  { [start chain] 
	    \chainin (m-1-1);
	    { [start branch=A] \chainin (m-2-1)
	        [join={node[right] {$\scriptstyle\alpha$}}];}

	    \chainin (m-1-2)  [join={node[above] {$\scriptstyle f$}}];
	    { [start branch=B] \chainin (m-2-2)
	        [join={node[right] {$\scriptstyle\beta$}}];}

	    \chainin (m-1-3) [join={node[above] {$\scriptstyle g$}}];
	    { [start branch=C] \chainin (m-2-3)
	        [join={node[right] {$\scriptstyle\gamma$}}];}

	    \chainin (m-1-4) [join={node[above] {$\scriptstyle h$}}];
	    { [start branch=D] \chainin (m-2-4)
	        [join={node[right] {$\scriptstyle\delta$}}];}

	    \chainin (m-1-5)  [join={node[above] {$\scriptstyle k$}}];}
  	    { [start branch=E] \chainin (m-2-5)
	        [join={node[right] {$\scriptstyle\varepsilon$}}];}

	  { [start chain] \chainin (m-2-1);
	    \chainin (m-2-2) [join={node[above] {$\scriptstyle f'$}}];
	    \chainin (m-2-3) [join={node[above] {$\scriptstyle g'$}}];
	    \chainin (m-2-4) [join={node[above] {$\scriptstyle h'$}}];
	    \chainin (m-2-5) [join={node[above] {$\scriptstyle k'$}}]; }
	\end{tikzpicture}
	\end{center}

	\begin{enumerate}
		\item If $\beta$ and $\delta$ are surjective and $\varepsilon$ is injective, then $\gamma$ is surjective.
		\item If $\beta$ and $\delta$ are injective and $\alpha$ is surjective, then $\gamma$ is injective.
		\item If $\alpha, \beta, \delta$ and $\varepsilon$ are isomorphisms, then $\gamma$ is an isomorphism.
	\end{enumerate}

\textbf{R Exercise 2.14}: Let $A \xrightarrow f B \xrightarrow g C$ be a sequence of module maps. Prove that $gf = 0$ if and only if $\im f \subseteq \ker g$.  Give an example of such a sequence that is not exact.
	\begin{proof}
		Suppose $gf = 0$, that is, $f(g(a)) = 0$ for all $a \in A$. Let $b \in \im f$ then by definition there exists $a \in A$ such that $f(a) = b$. But we know by hypothesis that $0 = g(f(a)) = g(b)$ so $b \in \ker g$. Conclude that $\im f \subseteq \ker g$. Conversely, suppose that $\im f \subseteq \ker g$. Let $a \in A$ and observe that $f(a) \in \im f$. By hypothesis $f(a) \in \ker g$ so $g(f(a)) = 0$. Since $a$ was arbitrary conclude $gf = 0$.
	\end{proof}
	Consider the sequence of module maps $\Z/4\Z \xrightarrow f \Z/3\Z \xrightarrow g \Z/2\Z$ where $f(\overline x) = 2 \overline x$ and $g(\overline y) = \overline y$. Observe that $\im f = \Z/3\Z$  and $\ker g = \{0\}$. Since $\im f \neq \ker g$ it follows that this is \textbf{not} an exact sequence.\\

\textbf{R Exercise 2.15}:
	\begin{enumerate}
		\item Prove that $f : M \to N$ is surjective if and only if $\coker f = \{0\}$.
			\begin{proof}
				Suppose $f : M \to N$ is surjective then for $n \in N$, there exists $m \in M$ such that $f(m) = n$. By definition $\coker f = M/\im f = M/M = 0$. Conversely, suppose that $\coker f = 0$, i.e., $M/\im f = 0$ implying that if $m + \im f \in M/\im f$ then $m + \im f = 0$ or equivalently $m \in \im f$. Since $m$ is arbitrary, conclude $M = \im f$ and hence $f$ is surjective by definition.
			\end{proof}
		\item If $f : M \to N$ is a map, prove that there is an exact sequence $$ 0 \rightarrow \ker f \rightarrow M \xrightarrow f N \rightarrow \coker f \rightarrow 0.$$
			\begin{proof}
				Define $h : \ker f \to M$ by $h(m) = m$, that is, map each element to itself. It follows immediately that $\im h = \ker f$. Define $g : N \to \coker f = N/\im f$ by $g(n) = n + \im f$, that is, the canonical/projection mapping. Observe that $\ker g = \im f$. Conclude that the following sequence is in fact exact: $$0 \xrightarrow{\text{identity}} \ker f \xrightarrow h M \xrightarrow f N \xrightarrow g \coker f \xrightarrow{\text{zero}}. \qedhere$$
			\end{proof}
	\end{enumerate}

\textbf{R Exercise 2.16}:
	\begin{enumerate}
		\item If $0 \rightarrow M \rightarrow 0$ is an exact sequence, prove that $M = \{0\}$.
			\begin{proof}
				Consider $0 \xrightarrow f M \xrightarrow g 0$. Since $f$ is surjective then for $m \in M$ there exists $x \in 0$ such that $f(x) = m$ but $x$ must be $0$ so $m = 0$.
			\end{proof}
		\item If $A \xrightarrow f B \xrightarrow g C \xrightarrow h D$ is an exact sequence, prove that $f$ is surjective if and only if $h$ is injective.
			\begin{proof}
				Suppose $f$ is surjective. Then $\im f = B = \ker g$ but this immediately implies that $\im g = 0 = \ker h$ so $h$ is injective by definitoin. Conversely, suppose $h$ is injective. Then $\ker h = 0 = \im g$ which immediately implies $\ker g = B = \im f$. Conclude by definition $f$ is surjective.
			\end{proof}
		\item Let $A \xrightarrow \alpha B \xrightarrow \beta C \xrightarrow \gamma D \xrightarrow \delta E$ be exact. If $\alpha$ and $\delta$ are isomorphisms, prove that $C = \{0\}$.
			\begin{proof}
				Observe that, by previous exercise, $\beta$ is surjective and $\gamma$ is injective so we have $\im \beta = C$ and $\ker \gamma = 0$. Result follows by exactness: $C = \im \beta = \ker \gamma = 0$. Conclude $C = \{0\}$.
			\end{proof}
	\end{enumerate}

\textbf{R Exercise 2.17}: If $A \xrightarrow f B \xrightarrow g C \xrightarrow h D \xrightarrow k E$ is exact, prove that there is an exact sequence $0 \rightarrow \coker f \xrightarrow \alpha C \xrightarrow \beta \ker k \rightarrow 0$, where $\alpha : b + \im f \mapsto g(b)$ and $\beta : c \mapsto h(c)$.
	\begin{proof}
		Observe that $\ker \beta = \{c \in C : \beta(c) = h(c) = 0\} = \ker h = \im g$ by exactness and since $\alpha$ can run through any $b \in B$ conclude $\im \alpha = \im g = \ker \beta$
	\end{proof}

\textbf{AM Proposition 2.10}: (\textit{Snake Lemma}) Let

	\begin{center}
	\begin{tikzpicture}
	  \matrix (m) [matrix of math nodes, row sep=3em, column sep=3em]
	    { 0 & M'  & M  & M''  & 0 \\
	      0 & N' & N & N'' & 0 \\ };
	  { [start chain] \chainin (m-1-1);
	    \chainin (m-1-2);
	    { [start branch=A] \chainin (m-2-2)
	        [join={node[right] {$\scriptstyle f'$}}];}
	    \chainin (m-1-3) [join={node[above] {$\scriptstyle g$}}];
	    { [start branch=B] \chainin (m-2-3)
	        [join={node[right] {$\scriptstyle f$}}];}
	    \chainin (m-1-4) [join={node[above] {$\scriptstyle h$}}];
	    { [start branch=C] \chainin (m-2-4)
	        [join={node[right] {$\scriptstyle f''$}}];}
	    \chainin (m-1-5); }
	  { [start chain] \chainin (m-2-1);
	    \chainin (m-2-2);
	    \chainin (m-2-3) [join={node[above] {$\scriptstyle g'$}}];
	    \chainin (m-2-4) [join={node[above] {$\scriptstyle h'$}}];
	    \chainin (m-2-5); }
	\end{tikzpicture}
	\end{center}

be a commutative diagram of $R$-modules and homomorphisms, with the rows exact. Then there exists a sequence $$0 \rightarrow \ker(f') \xrightarrow{\overline u} \ker(f) \xrightarrow{\overline v} \ker (f'') \xrightarrow d \coker(f') \xrightarrow {\overline u'} \coker (f) \xrightarrow{\overline v'} \coker(f'') \rightarrow 0$$ in which $\overline u$, $\overline v$ are restrictions of $u, v$, and $\overline u', \overline v'$ are induced by $u', v'$.
\end{document}




